using same lemma name as Hacl.Spec.EC.AddAndDouble2

code/curve25519/Hacl.Spec.EC.AddAndDouble3.fst
@@ -11,7 +11,6 @@ open Hacl.Spec.EC.AddAndDouble2
 
 #set-options "--initial_fuel 0 --max_fuel 0 --z3rlimit 10"
 
-
 val lemma_op_Star_Star_def_0: x:elem -> Lemma (Spec.Curve25519.(x ** 1 = x))
 #set-options "--initial_fuel 1 --max_fuel 1"
 let lemma_op_Star_Star_def_0 x = ()
@@ -44,7 +43,8 @@ val lemma_add_and_multiply: x_1:elem -> x_2:elem -> z_2:elem -> x_3:elem -> z_3:
     let z3 = x_1 *@ ((da -@ cb) *@ (da -@ cb)) in
     let x2 = aa *@ bb in
     let z2 = e *@ (aa +@ (121665 *@ e)) in
-    (x2, z2, x3, z3) == Spec.Curve25519.add_and_double x_1 x_2 z_2 x_3 z_3)
+    (Spec.Curve25519.Proj x2 z2, Spec.Curve25519.Proj x3 z3) ==
+      Spec.Curve25519.add_and_double x_1 (Spec.Curve25519.Proj x_2 z_2) (Spec.Curve25519.Proj x_3 z_3))
 let lemma_add_and_multiply x_1 x_2 z_2 x_3 z_3 =
   let a  = x_2 +@ z_2 in
   lemma_Star_Star a;
@@ -61,21 +61,13 @@ let lemma_add_and_multiply x_1 x_2 z_2 x_3 z_3 =
   lemma_Star_Star (da -@ cb)
 
 
-
-val fmonty_tot:
-  px:s_513 -> pz:s_513 ->
-  pqx:s_513 -> pqz:s_513 ->
-  qx:s_513 ->
-  Tot (t:(s_513 * s_513 * s_513 * s_513){
-    let x2 = selem (Mktuple4?._1 t) in
-    let z2 = selem (Mktuple4?._2 t) in
-    let x3 = selem (Mktuple4?._3 t) in
-    let z3 = selem (Mktuple4?._4 t) in
+val lemma_fmonty_split:   px:s_513 -> pz:s_513 -> pqx:s_513 -> pqz:s_513 -> qx:s_513 ->
+  Lemma (
+    let x2, z2, x3, z3 = fmonty_tot px pz pqx pqz qx in
+    let x2 = selem x2 in let z2 = selem z2 in let x3 = selem x3 in let z3 = selem z3 in
     let x_2 = selem px in let z_2 = selem pz in
     let x_3 = selem pqx in let z_3 = selem pqz in let x_1 = selem qx in
-    (x2, z2, x3, z3) == Spec.Curve25519.add_and_double x_1 x_2 z_2 x_3 z_3
-    })
-#reset-options "--initial_fuel 0 --max_fuel 0 --z3rlimit 10"
-let fmonty_tot px pz pqx pqz qx =
-  lemma_add_and_multiply (selem qx) (selem px) (selem pz) (selem pqx) (selem pqz);
-  fmonty_tot px pz pqx pqz qx
+    (Spec.Curve25519.Proj x2 z2, Spec.Curve25519.Proj x3 z3) ==
+      Spec.Curve25519.add_and_double x_1 (Spec.Curve25519.Proj x_2 z_2) (Spec.Curve25519.Proj x_3 z_3))
+let lemma_fmonty_split px pz pqx pqz qx =
+  lemma_add_and_multiply (selem qx) (selem px) (selem pz) (selem pqx) (selem pqz)
